some progress on deadlock

src/stuttering.lean
@@ -1,11 +1,11 @@
-import str init.data.set
+import str init.data.set data.set
 namespace operators
 open str 
 -- Type to know if some actions are available or if there is a deadlock
 universe u
 inductive completed (α : Type u)
 	| deadlock {} : completed
-	| some    : α → completed
+	| some   {} : α → completed
 
 -- Operator used to complete a STR by adding implicit transitions
 def add_implicit_transitions
@@ -36,22 +36,39 @@ def no_deadlock
   (str : STR C A)
 : Prop := 
   ∀ c, 
-    str.actions c ≠ ∅ 
-  ∧ ∀ a ∈ str.actions c, str.execute c a = ∅
+    (str.actions c).nonempty
+  ∧ ∃ a ∈ str.actions c, (str.execute c a).nonempty
 
+def has_deadlock 
+  (C A : Type)
+  (str : STR C A)
+: Prop := 
+  ∃ c, 
+    str.actions c = ∅ 
+  ∨ ∀ a ∈ str.actions c, str.execute c a = ∅
+
+def deadlock_configuration 
+  {C A : Type}
+  (str : STR C A)
+  (c : C)
+: Prop :=
+  str.actions c = ∅ 
+  ∨ ∀ a ∈ str.actions c, str.execute c a = ∅
+
+
+
+@[simp]
 def add_implicit_steps
   (C A : Type)
   (str : STR C A)
-  [∀ c, decidable (str.actions c = ∅)]
-  [∀ c, decidable (∀ (a : A), a ∈ str.actions c → str.execute c a = ∅)]
+  -- [∀ c, decidable (str.actions c = ∅)]
+  -- [∀ c, decidable (∀ (a : A), a ∈ str.actions c → str.execute c a = ∅)]
+  [∀ c, decidable (deadlock_configuration str c)]
 : STR C (completed A) :=
 {
   initial := str.initial,
   actions := λ c, 
-              if str.actions c = ∅ then
-                singleton completed.deadlock
-              else
-                if ∀ a ∈ str.actions c, str.execute c a = ∅ then 
+              if h : deadlock_configuration str c then 
                   singleton completed.deadlock
                 else
                   { x | ∀ a ∈ str.actions c, x = completed.some a },
@@ -61,21 +78,36 @@ def add_implicit_steps
         end 
 }
 
+
 theorem add_imp_rem_deadlock 
-  (C A : Type)
+  (C: Type)
+  (A: Type)
   (str : STR C A)
-  [∀ c, decidable (str.actions c = ∅)]
-  [∀ c, decidable (∀ (a : A), a ∈ str.actions c → str.execute c a = ∅)]
+  (deadlock : ¬ no_deadlock C A str)
+  -- [∀ c, decidable (str.actions c = ∅)]
+  -- [∀ c, decidable (∀ (a : A), a ∈ str.actions c → str.execute c a = ∅)]
+  [∀ c, decidable (deadlock_configuration str c)]
 : 
   no_deadlock C (completed A) (add_implicit_steps C A str)
 := 
-by {
-  unfold no_deadlock, intros, simp *,
-  split,rw add_implicit_steps, simp * at *, 
-  have h : (str.actions c = ∅), 
-    sorry, 
-    simp *, sorry,
-  intros, rw add_implicit_steps, simp *,  sorry,
-}
+begin
+  simp * at *, intro, simp at *, split_ifs, 
+    finish *, 
+  --   split, exact not_empty_when_no_deadlock C A str c h,
+  
+  --   revert h, simp at *, unfold deadlock_configuration, 
+  --   refine classical.skolem.mpr _, refine ex_of_psig _, refine ⟨_, _⟩, 
+  --   intro, exact completed.deadlock,
+    
+  -- refine imp_and_distrib.mpr _, split, 
+  -- revert deadlock, unfold no_deadlock,
+
+  -- simp * at *, intros, revert ᾰ_1, refine not_imp.mpr _, split, 
+  -- revert ᾰ, refine imp_or_distrib.mpr _, refine or.inl _, safe *, revert ᾰ_1,
+  -- -- hint, 
+  -- refine not_imp.mpr _, norm_num, revert ᾰ, exact set.not_nonempty_iff_eq_empty.mp, simp [not_nonempty_iff_eq_empty], 
+  
+  sorry,
+end
 
 end operators
